feat: rewrite translate_term to option term
TODO: finish rewriting the proofs to match the change

theories/Semantics.v
@@ -1,22 +1,36 @@
 From MetaCoq.Erasure.Typed Require Import ExAst Utils WcbvEvalAux.
 From MetaCoq.Erasure.Typed Require Import TypeAnnotations.
 From MetaCoq.Erasure.Typed Require Import Annotations.
-From MetaCoq.Erasure Require Import EAst.
+From MetaCoq.Erasure Require Import EAst EWellformed.
 From MetaCoq.Utils Require Import utils.
-From MetaCoq.Template Require Import Loader.
-From MetaCoq.ErasurePlugin Require Import Loader.
+
 From VTL Require Import PIR BigStepPIR Translation.
 
 Existing Instance EWcbvEval.default_wcbv_flags.
 
-Definition InSubset gt :=
-  match gt with
-  | tRel _
-  | tLambda _ _
-  | tApp (tLambda _ _) _ => True
-(* | some primitive value to replace vars with *)
-  | _ => False
-  end.
+Inductive InReflSubset (ctx : context) : EAst.term -> Prop :=
+  | RS_tBox : InReflSubset ctx tBox
+  | RS_tRel : forall n res,
+    nth_error ctx n = Some res ->
+    InReflSubset ctx (tRel n)
+  | RS_tLambda : forall na t,
+    InReflSubset ctx t ->
+    InReflSubset ctx (tLambda na t)
+.
+
+Inductive InSubset (ctx : context) : EAst.term -> Prop :=
+  | S_tBox : InSubset ctx tBox
+  | S_tRel : forall n res,
+    nth_error ctx n = Some res ->
+    InSubset ctx (tRel n)
+  | S_tLambda : forall na t,
+    InSubset ctx t ->
+    InSubset ctx (tLambda na t)
+  | S_tApp : forall t1 t2,
+    InSubset ctx t1 ->
+    InSubset ctx t2 ->
+    InSubset ctx (tApp t1 t2)
+.
 
 Definition gal_id :=
   tLambda (BasicAst.nNamed "x") (tRel 0).
@@ -24,90 +38,120 @@ Definition gal_id :=
 Import Coq.Strings.String.
 Local Open Scope string_scope.
 
+Notation "ctx p⊢ tl{ gt | ann_gt }" := (translate_term remap_env ctx gt ann_gt) (at level 100).
+Notation "ctx p⊢ { gt | ann_gt } '⇓ₚ' { gv | ann_gv }" :=
+  (forall pt pv,
+  (translate_term remap_env ctx gt ann_gt) = Some pt ->
+  (translate_term remap_env ctx gv ann_gv) = Some pv ->
+  (evaluatesTo pt pv))
+  (at level 50, gt, ann_gt, gv, ann_gv at next level).
+
 Ltac solve_pir_eval := split; [(eexists ; eauto using eval) | constructor].
-Ltac solve_err := simpl in *; contradiction.
+Ltac solve_inv_eval := intros pt pv Hgt Hgv; inversion Hgt; inversion Hgv; solve_pir_eval.
+Ltac solve_err := simpl in *; try contradiction; try discriminate.
 
 Lemma galEvalId : forall Σ, Σ e⊢ gal_id ⇓ gal_id.
 Proof.
   intros. eauto.
 Qed.
 
-Theorem id_correct_explicit : forall Σ, Σ e⊢ gal_id ⇓ gal_id ->
-  let gal_id' := (translate_term remap_env nil gal_id
-    (TArr (TConst <%% unit %%>) (TConst <%% unit %%>), (TConst <%% unit %%>))) in
-  gal_id' ⇓ gal_id'.
+Theorem id_correct_explicit : forall Σ, 
+  let ann := (TArr (TConst <%% unit %%>) (TConst <%% unit %%>), (TConst <%% unit %%>)) in
+  Σ e⊢ gal_id ⇓ gal_id ->
+  nil p⊢ {gal_id | ann} ⇓ₚ {gal_id | ann}.
 Proof with (eauto using eval).
-  intros.
-  unfold gal_id' in *.
-  simpl in *. split... constructor.
+  intros Σ ann ev.
+  unfold gal_id in *. simpl in *.
+  solve_inv_eval.
 Qed.
 
 Theorem id_correct_implicit : forall Σ ctx (ann : annots box_type gal_id),
-  let gal_id' := translate_term remap_env ctx gal_id ann in
   Σ e⊢ gal_id ⇓ gal_id ->
-  InSubset gal_id ->
-  ~ (isError gal_id') ->
-  gal_id' ⇓ gal_id'.
+  InSubset ctx gal_id ->
+  ctx p⊢ { gal_id | ann } ⇓ₚ { gal_id | ann }.
 Proof with (eauto using eval).
-  intros. simpl in gal_id'.
-  destruct ann eqn:Ea. destruct (decompose_arr b).
-  destruct l; try solve_err; 
-  unfold get_type in gal_id';
-  try solve_pir_eval;
-  try solve_err.
-  induction b1;
-  try solve_pir_eval;
-  try solve_err.
-  destruct (Env.with_default (UNDEFINED "NotInMap")
-  (Env.lookup remap_env
-  (bs_to_s Kernames.string_of_kername k)));
-  try solve_pir_eval;
-  try solve_err.
+  intros Σ ctx ann ev sub.
+  unfold gal_id in *.
+  destruct ann as [bt a]. rewrite unfold_lamAbs.
+  destruct (decompose_arr bt) as [[] _]; try discriminate.
+  destruct (get_type remap_env b). simpl.
+  - solve_inv_eval.
+  - discriminate.
 Qed.
 
-Theorem trans_lambda : forall ctx na t bt1 bt2 (ann : annots box_type t),
-  let lt := translate_term remap_env ctx (tLambda na t) (TArr bt1 bt2, ann) in
-  ~ (isError lt) ->
-  lt ⇓ lt.
+Theorem tl_lambda : forall ctx na t (ann : annots box_type (tLambda na t)),
+  ctx p⊢ { tLambda na t | ann} ⇓ₚ { tLambda na t | ann}.
 Proof with (eauto using eval).
-  intros.
-  simpl in lt. destruct (decompose_arr bt2).
-  - induction bt1; unfold get_type in lt;
-  try solve_pir_eval;
-  try solve_err.
-  (* this is fragile*)
-  destruct (Env.with_default (UNDEFINED "NotInMap")
-  (Env.lookup remap_env
-  (bs_to_s Kernames.string_of_kername k)));
-  try solve_pir_eval;
-  try solve_err.
-Qed.
-
-Theorem translation_correct : 
-  forall Σ ctx gt (ann : annots box_type gt),
-  let gt' := translate_term remap_env ctx gt ann in
-  Σ e⊢ gt ⇓ gt ->
-  InSubset gt ->
-  ~ isError gt' ->
-  gt' ⇓ gt'.
-Proof with (eauto using eval).
-  intros Σ ctx gt ann gt' ev sub nerr. 
-  destruct gt eqn:Egt; simpl in gt';
-  (* this gets rid of terms that are not implemented or give a trivial error *)
-  try solve_err.
-  (* - (* tBox => Constant, add this if tBox is in the subset *) try solve_pir_eval. *)
-  - (* tRel *) destruct (nth_error ctx n).
-    + destruct c. destruct decl_name.
-      * solve_err.
-      * split.
-        ** eexists. unfold gt'. admit. (* what to do in var case *)
-        ** unfold gt'. admit.
-    + solve_err.
-  - (* tLambda *) destruct ann eqn:Ea. destruct b; simpl in gt';
-    try solve_err.
-    + apply trans_lambda. simpl. destruct (decompose_arr b2).
-      destruct (get_type remap_env b1)...
-  - (*tApp*) destruct t1; simpl in sub; try contradiction.
-    (* lemma that is valid for all types that make sense *)
-    simpl in *. admit.
+  intros ctx na t ann.
+  destruct ann as [bt a]. rewrite unfold_lamAbs.
+  destruct (decompose_arr bt) as [[] _]; try discriminate.
+  destruct (get_type remap_env b) as [ty|]; try discriminate.
+  destruct t; try discriminate; simpl.
+  - solve_inv_eval.
+  - destruct (nth_error (vass (BasicAst.nNamed (s_to_bs get_name na)) :: ctx) n).
+    destruct c. destruct decl_name; try discriminate. simpl.
+    + solve_inv_eval.
+    + discriminate.
+  - destruct a as [[] a']; try discriminate.
+    + simpl. destruct (decompose_arr codom).
+    destruct (get_type remap_env dom) as [ty'|]; try discriminate. admit.
+  - admit.
 Admitted.
+
+(* use unfold lemmas, translate app = *)
+Theorem refl_tl_correct : forall Σ ctx gt (ann : annots box_type gt),
+  Σ e⊢ gt ⇓ gt ->
+  InReflSubset ctx gt ->
+  ctx p⊢ { gt | ann} ⇓ₚ {gt | ann}.
+Proof with (eauto using eval).
+  intros Σ ctx gt ann ev rsub.
+  destruct rsub.
+  - (* TBox *) solve_inv_eval.
+  - (* tRel, either an error or ev is invalid *) 
+    simpl in *. destruct (nth_error ctx n). destruct c. destruct decl_name.
+    + discriminate.
+    + now inversion ev.
+    + discriminate.
+  - (* tLambda *) destruct ann as [bt a]. rewrite unfold_lamAbs.
+  destruct (decompose_arr bt). destruct l; try discriminate.
+  destruct (get_type remap_env b0) as [ty|]; try discriminate.
+  destruct ty eqn:Ety; simpl; try discriminate. admit.
+Qed.
+
+(*Definition id_app := tApp
+  (tLambda (BasicAst.nNamed "x"%bs) (tRel 0)) (tBox).
+
+Theorem id_app_correct : forall ctx (ann : annots box_type id_app),
+  ~ (ctx p⊢ tl_err{id_app | ann}) ->
+  ctx p⊢ {id_app | ann} ⇓ₚ {tBox | TBox}.
+Proof with (eauto using eval).
+  intros ctx ann nerr.
+  unfold id_app. destruct ann. destruct p. rewrite unfold_app. split.
+  - eexists. eapply E_Apply... 
+  (* destruct ann as [annv [[dom codom] bt]]; try solve_err.
+  destruct (decompose_arr dom); destruct l; try solve_err.
+  unfold not in nerr. simpl in nerr. destruct nerr. left. trivial.
+  destruct (get_type remap_env b0); split. 
+  - eexists. eapply E_Apply... simpl...
+  - constructor.
+  - eexists. admit. (* it sees λ(x : tt, x) x as valid*)
+  - constructor.
+  - unfold not in nerr. simpl in nerr. destruct nerr. left. trivial.
+  - constructor. *)
+Admitted.
+
+Theorem stlc_correct : forall Σ ctx 
+  gt (ann_gt : annots box_type gt)
+  gv (ann_gv : annots box_type gv),
+  Σ e⊢ gt ⇓ gv ->
+  InSubset ctx gt ->
+  ~ (ctx p⊢ tl_err{gt | ann_gt}) ->
+  InSubset ctx gv ->
+  ~ (ctx p⊢ tl_err{gv | ann_gv}) ->
+  ctx p⊢ {gt | ann_gt} ⇓ₚ {gv | ann_gv}.
+Proof with (eauto using eval).
+  intros Σ ctx gt ann_gt gv ann_gv.
+  intros ev sub_gt nerr_gt sub_gv nerr_gv.
+  (* main proof, set up useful lemmas first *)
+  (* refl cases*)
+Admitted. *)
